i think i've been doing this completely wrong.  the statement of completeness should just be slightly weaker: we can derive any meta fatcs that are _finite_

src/Dataflow.v
@@ -1497,38 +1497,205 @@ Section DistributedDatalog.
       incl hyps' facts ->
       Exists (fun r => rule_impl r f hyps') p ->
       In f (step_everybody p facts).
-  
-  Definition no_R_cycles R (r : rule) :=
-    match r with
-    | normal_rule concls hyps =>
-        In R (map fact_R concls) ->
-        In R (map fact_R hyps) ->
-        False
-    | agg_rule _ _ _ => True (*TODO*)
-    | meta_rule _ _ _ => True
-    end.
 
+  Definition is_normal_dfact f :=
+    match f with
+    | normal_dfact _ _ => true
+    | meta_dfact _ _ _ => false
+    end.
+  
+  Definition rel_ofd f :=
+    match f with
+    | normal_dfact R _ => R
+    | meta_dfact R _ _ => R
+    end.           
+  
   Definition add_facts ns fs :=
     {| known_facts := fs ++ ns.(known_facts);
       msgs_received := ns.(msgs_received);
-      msgs_sent := ns.(msgs_sent); |}.
+      msgs_sent := fun R =>
+                     ns.(msgs_sent) R + length (filter (fun f => is_normal_dfact f && rel_eqb (rel_ofd f) R) fs); |}.
 
-  Definition add_facts_at_node g n fs :=
-    {| node_states := fun n' => if node_eqb n n' then
-                               add_facts (g.(node_states) n) fs
-                             else
-                               g.(node_states) n;
-      travellers := g.(travellers);
-      input_facts := g.(input_facts); |}.
-
-  (* Definition normal_dfact_of_fact (f : fact) : option dfact := *)
-  (*   match f with *)
-  (*   | normal_fact R args => Some (normal_dfact R args) *)
-  (*   |  *)
+  Definition equiv_fun {A B : Type} (f f' : A -> B) :=
+    forall x, f x = f' x.
   
+  Definition equiv_node ns ns' :=
+    ns.(known_facts) = ns'.(known_facts) /\
+      equiv_fun ns.(msgs_received) ns'.(msgs_received) /\
+      equiv_fun ns.(msgs_sent) ns'.(msgs_sent).
+
+  Definition equiv_graph g g' :=
+    g.(travellers) = g'.(travellers) /\
+      g.(input_facts) = g'.(input_facts) /\
+      forall n, equiv_node (g.(node_states) n) (g'.(node_states) n).
+
+  Definition add_facts_at_node g n fs g' :=
+    equiv_graph
+      g'
+      {| node_states := fun n' => if node_eqb n n' then
+                                 add_facts (g.(node_states) n) fs
+                               else
+                                 g.(node_states) n';
+        travellers := flat_map (fun f => map (fun n' => (n', f)) all_nodes) fs ++ g.(travellers);
+        input_facts := g.(input_facts); |}.
+  Hint Unfold add_facts_at_node equiv_graph equiv_node equiv_fun : core.
+
+  Lemma expect_num_R_facts_knows_everything g n R args :
+    sane_graph g ->
+    good_inputs g.(input_facts) ->
+    expect_num_R_facts R (g.(node_states) n).(known_facts)
+                                               ((g.(node_states) n).(msgs_received) R) ->
+    knows_fact g (normal_dfact R args) ->
+    In (normal_dfact R args) (g.(node_states) n).(known_facts).
+  Proof.
+    intros Hsane Hinp HR Hargs.
+    pose proof expect_num_R_facts_no_travellers as H'.
+    epose_dep H'. specialize (H' ltac:(eassumption) ltac:(eassumption) ltac:(eassumption)).
+    destruct Hsane as (_&_&_&_&Heverywhere&_).
+    specialize (Heverywhere _ ltac:(eassumption)).
+    edestruct Heverywhere; [|eassumption].
+    exfalso. eauto.
+  Qed.
+
+  Lemma equiv_node_known_facts ns ns' :
+    equiv_node ns ns' ->
+    ns.(known_facts) = ns'.(known_facts).
+  Proof. cbv [equiv_node]. intros. fwd. auto. Qed.
+  
+  Lemma equiv_node_msgs_received ns ns' R :
+    equiv_node ns ns' ->
+    ns.(msgs_received) R = ns'.(msgs_received) R.
+  Proof. cbv [equiv_node]. intros. fwd. auto. Qed.
+  
+  Lemma known_facts_add_facts ns fs :
+    (add_facts ns fs).(known_facts) = fs ++ ns.(known_facts).
+  Proof. destruct ns. reflexivity. Qed.
+
+  Lemma msgs_received_add_facts ns fs :
+    (add_facts ns fs).(msgs_received) = ns.(msgs_received).
+  Proof. destruct ns. reflexivity. Qed.
+
+  Lemma no_learning_inputs g n R args :
+    can_learn_normal_fact_at_node (rules n) (node_states g n) R args ->
+    is_input R = false.
+  Proof.
+    intros H. cbv [can_learn_normal_fact_at_node] in H. fwd.
+    cbv [good_rules] in rules_good. specialize (rules_good n).
+    rewrite Forall_forall in rules_good.
+    specialize (rules_good _ ltac:(eassumption)).
+    destruct r; fwd; simpl in rules_good.
+    - apply Exists_exists in Hp1p0. fwd. invert Hp1p0p1.
+      apply Lists.List.Forall_map in rules_good.
+      rewrite Forall_forall in rules_good.
+      apply rules_good. assumption.
+    - assumption.
+    - contradiction.
+  Qed.
+  
+  (*this has something to do with can_learn_normal_fact_at_node_relevant_facts_incl*)
+  Lemma step_to_add_normal_facts_at_node g n fs :
+    meta_facts_correct rules g ->
+    Forall (fun f => is_normal_dfact f = true) fs ->
+    Forall (should_learn_fact_at_node (rules n) n (g.(node_states) n)) fs ->
+    exists g',
+      comp_step^* g g' /\
+        add_facts_at_node g n fs g'.
+  Proof.
+    intros Hmf. induction 1; intros Hshould.
+    - exists g. split; auto. cbv [add_facts_at_node equiv_graph]. simpl. ssplit; auto.
+      intros n'. destr (node_eqb n n'); auto.
+    - invert Hshould. specialize (IHForall ltac:(assumption)). fwd.
+      destruct x; simpl in *; try congruence. fwd.
+      cbv [add_facts_at_node equiv_graph] in IHForallp1.
+      simpl in IHForallp1. fwd.
+      eexists. split.
+      + eapply trc_trans; [eassumption|].
+        eapply TrcFront; [|apply TrcRefl].
+        specialize (IHForallp1p2 n). destr (node_eqb n n); [|congruence].
+        eapply LearnFact with (f := normal_dfact _ _).
+        simpl. split.
+        { intros num Hnum. 
+          erewrite equiv_node_known_facts in Hnum by eassumption.
+          eapply H3p0.
+          rewrite known_facts_add_facts in Hnum. apply in_app_iff in Hnum.
+          destruct Hnum as [Hnum|Hnum]; [|exact Hnum].
+          rewrite Forall_forall in H0. apply H0 in Hnum. simpl in Hnum. congruence. }
+        instantiate (1 := nf_args).
+        cbv [can_learn_normal_fact_at_node] in *. fwd. exists r. split; [eassumption|].
+        destruct r; fwd.
+        -- do 2 eexists. split; [eassumption|]. split; [eassumption|].
+           erewrite equiv_node_known_facts by eassumption.
+           rewrite known_facts_add_facts.
+           intros. apply in_app_iff. auto.
+        -- erewrite equiv_node_known_facts by eassumption.
+           erewrite equiv_node_msgs_received by eassumption.
+           rewrite msgs_received_add_facts. split.
+           { eapply expect_num_R_facts_incl; [eassumption|].
+             rewrite known_facts_add_facts. auto with incl. }
+           eexists. ssplit; eauto. rewrite known_facts_add_facts.
+           destruct H3p1p1p1p0 as [ils1 ils2]. split; [|assumption].
+           intros x. rewrite in_app_iff. split.
+           2: { intros. right. apply ils1. assumption. }
+           intros [Hx|Hx].
+           2: { apply ils1. assumption. }
+           rewrite Forall_forall in H4. specialize (H4 _ Hx). simpl in H4.
+           destruct H4 as [_ H4]. apply ils1.
+           cbv [meta_facts_correct] in Hmf. specialize (Hmf n).
+           cbv [meta_facts_correct_at_node] in Hmf.
+           cbv [expect_num_R_facts] in H3p1p1p0.
+           pose proof H4 as H4'.
+           apply no_learning_inputs in H4. rewrite H4 in H3p1p1p0.
+           fwd. apply Forall2_forget_r in H3p1p1p0p0.
+           rewrite Forall_forall in H3p1p1p0p0. specialize (H3p1p1p0p0 n).
+           specialize' H3p1p1p0p0.
+           { destruct Hall_nodes as [H' _]. apply H'. constructor. }
+           fwd. specialize (Hmf _ _ ltac:(eassumption)). destruct Hmf as [_ Hmf].
+           apply Hmf. assumption.
+        -- contradiction.
+      + cbv [add_facts_at_node equiv_graph]. simpl. ssplit.
+        -- rewrite <- app_assoc. f_equal. assumption.
+        -- assumption.
+        -- intros n'. specialize (IHForallp1p2 n'). destr (node_eqb n n'); auto.
+           cbv [equiv_node]. simpl.
+           erewrite equiv_node_known_facts by eassumption.
+           rewrite known_facts_add_facts. split; [reflexivity|].
+           split.
+           { cbv [equiv_node] in IHForallp1p2. fwd. auto. }
+           cbv [equiv_fun]. intros R.
+           cbv [equiv_node] in IHForallp1p2. fwd. do 2 rewrite IHForallp1p2p2.
+           destr (rel_eqb nf_rel R); simpl; lia.
+  Qed.
+
+  Definition normal_dfacts_of_facts : list fact -> list dfact :=
+    flat_map (fun f => match f with
+                    | normal_fact R args => [normal_dfact R args]
+                    | meta_fact _ _ => []
+                    end).
+
+  Definition normal_facts_of_dfacts : list dfact -> list fact :=
+    flat_map (fun f => match f with
+                    | normal_dfact R args => [normal_fact R args]
+                    | meta_dfact _ _ _ => []
+                    end).
+
+  Lemma should_learn_fact_at_node_em rules0 n ns f :
+    should_learn_fact_at_node rules0 n ns f \/ ~should_learn_fact_at_node rules0 n ns f.
+  Proof. apply Classical_Prop.classic. Qed.
+
+  Lemma add_facts_at_node_same_msgs_received g n fs g' :
+    add_facts_at_node g n fs g' ->
+    same_msgs_received g g'.
+  Proof. Admitted.
+
+  Lemma can_filter_prop {X : Type} (l : list X) P :
+    Forall (fun x => P x \/ ~P x) l ->
+    exists l',
+    forall x, In x l' <-> In x l /\ P x.
+  Proof. Admitted.
+    
   Lemma node_can_find_all_conclusions g n R :
-    (* Forall good_rule p -> *)
-    (* Forall (no_R_cycles R) p -> *)
+    meta_facts_correct rules g ->
+    Forall good_rule p ->
     exists g',
       comp_step^* g g' /\
         (forall args,
@@ -1536,16 +1703,33 @@ Section DistributedDatalog.
             In (normal_dfact R args) (known_facts (node_states g' n))) /\
         same_msgs_received g g'.
   Proof.
-    (* intros Hp Hl. *)
-    (* exists (add_facts_at_node g n (flat_map (fun f => *)
-    (*                                       match f with *)
-    (*                                       | normal_fact R' args => *)
-    (*                                           if rel_eqb R R' then *)
-    (*                                             [normal_dfact R' args] *)
-    (*                                           else *)
-    (*                                             [] *)
-    (*                                       | _ => [] *)
-    (*                                       end))). *)
+    intros Hmf Hp.
+    assert (Hor : (fun P => P \/ ~P) (exists num, In (meta_dfact R (Some n) num) (known_facts (node_states g n)))).
+    { apply Classical_Prop.classic. }
+    simpl in Hor. destruct Hor as [Hor|Hor].
+    { fwd. intros. exists g. split; [auto|]. split; [|cbv [same_msgs_received]; auto].
+      intros. apply Hmf in Hor. destruct Hor as [_ Hor]. apply Hor. assumption. }
+    set (new_facts := normal_dfacts_of_facts (filter (fun f => rel_eqb (rel_of f) R) (step_everybody (rules n) (normal_facts_of_dfacts (g.(node_states) n).(known_facts))))).
+    pose proof step_to_add_normal_facts_at_node as H'.
+    pose proof (can_filter_prop new_facts (should_learn_fact_at_node (rules n) n (g.(node_states) n))) as H''.
+    specialize' H''.
+    { apply Forall_forall. intros ? _. apply should_learn_fact_at_node_em. }
+    destruct H'' as (new_facts'&H'').
+    specialize (H' g n new_facts' ltac:(assumption)). specialize' H'.
+    { eapply incl_Forall.
+      - cbv [incl]. intros f Hf. apply H'' in Hf. fwd. eassumption.
+      - subst new_facts. cbv [normal_dfacts_of_facts]. apply Forall_flat_map.
+        apply Forall_filter. intros f. destruct f; auto. }
+    specialize' H'.
+    { apply Forall_forall. intros f Hf. apply H'' in Hf. fwd. assumption. }
+    fwd. eexists. split; [eassumption|]. split.
+    2: { eapply add_facts_at_node_same_msgs_received. eassumption. }
+    intros args Hargs.
+    cbv [add_facts_at_node] in H'p1. cbv [equiv_graph] in H'p1. simpl in *. fwd.
+    specialize (H'p1p2 n).
+    erewrite equiv_node_known_facts by eassumption.
+    destr (node_eqb n n); [|congruence].
+    rewrite known_facts_add_facts. apply in_app_iff. left. apply H''. simpl.
   Admitted.
 
   Lemma receive_fact_at_node_impl ns f f0 :
@@ -1611,23 +1795,6 @@ Section DistributedDatalog.
        eapply Htrav. rewrite Hf0. apply in_app_iff. simpl. eauto.
   Qed.
 
-  Lemma no_learning_inputs g n R args :
-    can_learn_normal_fact_at_node (rules n) (node_states g n) R args ->
-    is_input R = false.
-  Proof.
-    intros H. cbv [can_learn_normal_fact_at_node] in H. fwd.
-    cbv [good_rules] in rules_good. specialize (rules_good n).
-    rewrite Forall_forall in rules_good.
-    specialize (rules_good _ ltac:(eassumption)).
-    destruct r; fwd; simpl in rules_good.
-    - apply Exists_exists in Hp1p0. fwd. invert Hp1p0p1.
-      apply Lists.List.Forall_map in rules_good.
-      rewrite Forall_forall in rules_good.
-      apply rules_good. assumption.
-    - assumption.
-    - contradiction.
-  Qed.
-  
   Lemma knows_meta_fact_step_learns_nothing g g' R S args :
     sane_graph g ->
     knows_datalog_fact g (meta_fact R S) ->
@@ -1733,23 +1900,6 @@ Section DistributedDatalog.
         specialize (Hp0 n'). specialize' Hp0.
         { apply H'. constructor. }
         fwd. eauto.
-  Qed.
-
-  Lemma expect_num_R_facts_knows_everything g n R args :
-    sane_graph g ->
-    good_inputs g.(input_facts) ->
-    expect_num_R_facts R (g.(node_states) n).(known_facts)
-                                               ((g.(node_states) n).(msgs_received) R) ->
-    knows_fact g (normal_dfact R args) ->
-    In (normal_dfact R args) (g.(node_states) n).(known_facts).
-  Proof.
-    intros Hsane Hinp HR Hargs.
-    pose proof expect_num_R_facts_no_travellers as H'.
-    epose_dep H'. specialize (H' ltac:(eassumption) ltac:(eassumption) ltac:(eassumption)).
-    destruct Hsane as (_&_&_&_&Heverywhere&_).
-    specialize (Heverywhere _ ltac:(eassumption)).
-    edestruct Heverywhere; [|eassumption].
-    exfalso. eauto.
   Qed.
 
   Lemma hmfs_unique Q R S S' :
@@ -1886,12 +2036,6 @@ Section DistributedDatalog.
     constructor; auto. intros. rewrite <- H1. auto.
   Qed.
 
-  Definition rel_ofd f :=
-    match f with
-    | normal_dfact R _ => R
-    | meta_dfact R _ _ => R
-    end.           
-  
   Lemma graph_correct_for_preserved g g' R :
     sane_graph g ->
     (forall f, rel_ofd f = R ->
@@ -2276,7 +2420,9 @@ Section DistributedDatalog.
       
       specialize (Hg3 g2 n target_rel).
       destruct Hg3 as (g3&Hg3&Hhyps3a&Hhyps3b).
-      
+      { admit. }
+      { admit. }
+      clear Hhyps3a.
       eexists.
       split.
       { eapply Relations.trc_trans.
